Define quote_exp, though not perfectly
The definition of quote_exp_aux still contains remnants from the
recursive function package. They should not be there, but I'm not sure
if they will actually cause problems in proofs later or not.

botworld_quoteScript.sml
@@ -4,7 +4,19 @@ val _ = new_theory"botworld_quote";
 
 val (quote_num_aux_def,quote_num_def) = mk_quote NONE ``:num``
 val (quote_level_aux_def,quote_level_def) = mk_quote NONE ``:level``
+
 val (quote_prod_aux_def,quote_prod_def) = mk_quote (SOME(["q1","q2"],["t1","t2"])) ``:'a # 'b``
+
+val quote_prod_aux_cong = Q.store_thm("quote_prod_aux_cong",
+  `∀xy1 xy2 qta1 qtb1 qta2 qtb2.
+   xy1 = xy2 ∧
+   (∀q1 t1 q2 t2 x1. qta1 = (q1,t1) ∧ qta2 = (q2,t2) ∧ x1 = FST xy1 ⇒ t1 = t2 ∧ q1 x1 = q2 x1) ∧
+   (∀q1 t1 q2 t2 y1. qtb1 = (q1,t1) ∧ qtb2 = (q2,t2) ∧ y1 = SND xy1 ⇒ t1 = t2 ∧ q1 y1 = q2 y1)
+   ⇒
+   quote_prod_aux (qta1,qtb1) xy1 = quote_prod_aux (qta2,qtb2) xy2 `,
+  rpt Cases \\ rw[quote_prod_aux_def]);
+val _ = DefnBase.export_cong "quote_prod_aux_cong";
+
 val (quote_list_aux_def,quote_list_def) = mk_quote (SOME(["q"],["t"])) ``:'a list``
 
 val quote_list_aux_cong = Q.store_thm("quote_list_aux_cong",
@@ -36,8 +48,16 @@ val quote_t_aux_def = save_thm("quote_t_aux_def",
     quote_t_aux_def |> REWRITE_RULE[GSYM quote_list_is_aux,ETA_AX])
 
 val (quote_spec_aux_def,quote_spec_def) = mk_quote NONE ``:spec``
-val (quote_option_aux_def,quote_option_def) = mk_quote (SOME(["q"],["t"])) ``:'a option``
 val _ = overload_on("quote_specs",``quote_list quote_spec``)
+
+val (quote_option_aux_def,quote_option_def) = mk_quote (SOME(["q"],["t"])) ``:'a option``
+
+val quote_option_aux_cong = Q.store_thm("quote_option_aux_cong",
+  `∀o1 o2 q1 q2 t1 t2.
+   o1 = o2 ∧ t1 = t2 ∧ (∀x. o1 = SOME x ⇒ q1 x = q2 x)
+   ⇒ quote_option_aux (q1,t1) o1 = quote_option_aux (q2,t2) o2`,
+  Cases \\ simp[quote_option_aux_def]);
+val _ = DefnBase.export_cong"quote_option_aux_cong";
 
 val quote_int_aux_def = Define `quote_int_aux i = if i < 0i
                                                   then Comb ^(term_to_deep ``int_neg``)
@@ -63,12 +83,65 @@ val (quote_opb_aux_def,quote_opb_def) = mk_quote NONE ``:opb``
 val (quote_op_aux_def,quote_op_def) = mk_quote NONE ``:op``
 val (quote_lop_aux_def,quote_lop_def) = mk_quote NONE ``:lop``
 
+val quote_option_is_aux = Q.prove(
+  `FST (quote_option qt) z = quote_option_aux qt z`,
+  Cases_on`qt`\\rw[quote_option_def]);
+
+val _ = aux_rws := concl quote_option_is_aux :: !aux_rws
+
 (*
-val _ = mk_quote_tac := (wf_rel_tac `measure exp_size` \\ rpt conj_tac \\ simp[])
+val _ = aux_rws := tl (!aux_rws)
+*)
+
+(*
+val FST_cong = Q.store_thm("FST_cong",
+  `x1 = x2 ⇒
+   FST (x1,y1) = FST (x2,y2)`,rw[])
+val _ = DefnBase.export_cong"FST_cong";
+
+val SND_cong = Q.store_thm("SND_cong",
+  `y1 = y2 ⇒
+   SND (x1,y1) = SND (x2,y2)`,rw[])
+val _ = DefnBase.export_cong"SND_cong";
+*)
+
+val quote_prod_split1 = Q.prove(
+  `quote_prod x = (quote_prod_aux x, Pair (SND(FST x)) (SND(SND x)))`,
+  PairCases_on`x`\\rw[quote_prod_def]);
+
+val quote_prod_split2 = Q.prove(
+  `quote_prod (x,y) = (quote_prod_aux (x,y), Pair (SND x) (SND y))`,
+  PairCases_on`x`\\PairCases_on`y`\\rw[quote_prod_def]);
+
+val quote_prod_split3 = Q.prove(
+  `quote_prod (x,(y,z)) = (quote_prod_aux (x,(y,z)), Pair (SND x) z)`,
+  PairCases_on`x`\\rw[quote_prod_def]);
+
+val quote_prod_split4 = Q.prove(
+  `quote_prod ((x,y),z) = (quote_prod_aux ((x,y),z), Pair y (SND z))`,
+  PairCases_on`z`\\rw[quote_prod_def]);
+
+val _ = aux_rws :=
+  concl quote_prod_split4 ::
+  concl quote_prod_split3 ::
+  concl quote_prod_split2 ::
+  concl quote_prod_split1 ::
+  !aux_rws
+
+val _ = mk_quote_tac := (
+  wf_rel_tac `measure exp_size` \\ rpt conj_tac \\ simp[]
+  \\ gen_tac \\ Induct \\ rw[] \\ simp[astTheory.exp_size_def] \\ res_tac \\ simp[astTheory.exp_size_def]);
 
 val (quote_exp_aux_def,quote_exp_def) = mk_quote NONE ``:exp``
-*)
-val quote_exp = Define `quote_exp = (ARB:exp->term,ARB:type) (* TODO *)`
+val quote_exp_aux_def = save_thm("quote_exp_aux_def",
+    quote_exp_aux_def |>
+    REWRITE_RULE[ETA_AX,
+         GSYM quote_list_is_aux,
+         GSYM quote_option_is_aux,
+         GSYM quote_prod_split4,
+         GSYM quote_prod_split3,
+         GSYM quote_prod_split2,
+         GSYM quote_prod_split1]); (* TODO: remove RESTRICT *)
 
 val (quote_dec_aux_def,quote_dec_def) = mk_quote NONE ``:dec``
 val _ = overload_on("quote_decs",``quote_list quote_dec``)
@@ -76,9 +149,6 @@ val _ = overload_on("quote_decs",``quote_list quote_dec``)
 val (quote_top_aux_def,quote_top_def) = mk_quote NONE ``:top``
 
 val (quote_command_aux_def,quote_command_def) = mk_quote NONE ``:command``
-
-val quote_top_def = Define`
-  quote_top = (ARB:top->term,ARB:type) (* TODO *)`;
 
 val _ = overload_on("quote_prog",``quote_list quote_top``);
 
